src/FcEtt/ext_subst.v
@@ -21,7 +21,7 @@ Qed.
 
 Lemma binds_to_PropWff: forall G0 A B T R c,
     Ctx G0 ->
-    binds c (Co (Eq A B T R)) G0 -> PropWff G0 (Eq A B T R).
+    binds c (Co (Eq A B T R)) G0 -> PropWff G0 (Eq A B T R) Phm.
 Proof.
   induction G0; auto; try done.
   intros A B T R c H H0.
@@ -30,7 +30,7 @@ Proof.
   - case H0; try done.
     move => h0.
     inversion H; subst.
-    have:   PropWff ( G0) (Eq A B T R). 
+    have:   PropWff ( G0) (Eq A B T R) Phm. 
     apply (IHG0 _ _ _ _ c H4); eauto.
     move => h1.
     rewrite_env (nil ++ [(a, Tm A0 R0)] ++ G0).
@@ -94,10 +94,10 @@ Proof.
 Qed.
 
 Lemma co_subst_fresh :
-forall G phi a0 x s,
-  PropWff G phi -> Ctx ((x ~ s) ++ G) -> tm_subst_tm_constraint a0 x phi = phi.
+forall G phi a0 x s R ,
+  PropWff G phi R -> Ctx ((x ~ s) ++ G) -> tm_subst_tm_constraint a0 x phi = phi.
 Proof.
-  intros G phi a0 x s H H0.
+  intros G phi a0 x s R H H0.
   apply tm_subst_tm_constraint_fresh_eq.
   move: (ProfWff_context_fv H) => ?. split_hyp.
   inversion H0; subst; auto.
@@ -221,17 +221,17 @@ Lemma tm_substitution_mutual :
                       Typing (map (tm_subst_tm_sort a x) F ++ G)
                              (tm_subst_tm_tm a x b)
                              (tm_subst_tm_tm a x B) R) /\
-    (forall G0 phi (H : PropWff G0 phi),
+    (forall G0 phi R (H : PropWff G0 phi R),
         forall G a A R', Typing G a A R' ->
                  forall F x, G0 = (F ++ (x ~ (Tm A R')) ++ G) ->
                         PropWff (map (tm_subst_tm_sort a x) F ++ G)
-                                (tm_subst_tm_constraint a x phi)) /\
-    (forall G0 D p1 p2 (H : Iso G0 D p1 p2),
+                                (tm_subst_tm_constraint a x phi) R) /\
+    (forall G0 D p1 p2 R (H : Iso G0 D p1 p2 R ),
         forall G a A R', Typing G a A R' ->
                  forall F x, G0 = (F ++ (x ~ (Tm A R')) ++ G) ->
                 Iso (map (tm_subst_tm_sort a x) F ++ G) D
                     (tm_subst_tm_constraint a x p1)
-                    (tm_subst_tm_constraint a x p2)) /\
+                    (tm_subst_tm_constraint a x p2) R) /\
     (forall G0 D A B T R'' (H : DefEq G0 D A B T R''),
        forall G a A0 R', Typing G a A0 R' ->
                  forall F x, G0 = (F ++ (x ~ (Tm A0 R')) ++ G) ->
@@ -287,7 +287,7 @@ Proof. eapply typing_wff_iso_defeq_mutual;
     erewrite (tm_subst_fresh_2 _ h0); auto.
     erewrite (tm_subst_fresh_1 _ h0); auto. eauto.
     erewrite (tm_subst_fresh_1 _ h0); auto.
-  - eapply E_TyCast; try eapply DefEq_weaken_available; eauto.
+(*   - eapply E_TyCast; try eapply DefEq_weaken_available; eauto. *)
   - destruct (c == x).
     + subst.
       apply binds_mid_eq in b0; auto; try done.
@@ -301,17 +301,17 @@ Proof. eapply typing_wff_iso_defeq_mutual;
            by apply (H _ _ A0 R').
          have: Ctx ([(x, Tm A0 R')] ++ G0) by apply (Ctx_strengthen _ F); auto.
          inversion 1; subst.
-         have: PropWff G0 (Eq a b A R) by apply (binds_to_PropWff _ _ _ _ c); auto.
+         have: PropWff G0 (Eq a b A R) Phm by apply (binds_to_PropWff _ _ _ _ c); auto.
          inversion 1; subst.
          repeat rewrite tm_subst_tm_tm_fresh_eq; auto.
          -- move: (Typing_context_fv H11) => ?. split_hyp. auto.
+         -- move: (Typing_context_fv H12) => ?. split_hyp. auto.
          -- move: (Typing_context_fv H11) => ?. split_hyp. auto.
-         -- move: (Typing_context_fv H9) => ?. split_hyp. auto.
   - eapply E_Beta; eauto.
     eapply Beta_tm_subst; eauto with lc.
   - eapply E_EqConv; eauto 2.
     eapply DefEq_weaken_available; eauto.
-  - eapply E_CastCong; eauto.
+(*   - eapply E_CastCong; eauto. *)
   - destruct  F; try done.
   - induction F; try done.
     simpl; simpl in H2.
@@ -370,18 +370,18 @@ Lemma co_substitution_mutual :
           G0 = (F ++ (c ~ Co (Eq A1 A2 T R') ) ++ G)
           -> DefEq G D A1 A2 T R'
           -> Typing (map (co_subst_co_sort g_Triv c) F ++ G) (co_subst_co_tm g_Triv c b) (co_subst_co_tm g_Triv c B) R) /\
-    (forall G0 phi (H : PropWff G0 phi),
+    (forall G0 phi R (H : PropWff G0 phi R),
         forall G D A1 A2 T R' F c,
           G0 = (F ++ (c ~ Co (Eq A1 A2 T R') ) ++ G)
           -> DefEq G D A1 A2 T R'
-          -> PropWff (map (co_subst_co_sort g_Triv c) F ++ G) (co_subst_co_constraint g_Triv c phi)) /\
-    (forall G0 D0 p1 p2 (H : Iso G0 D0 p1 p2),
+          -> PropWff (map (co_subst_co_sort g_Triv c) F ++ G) (co_subst_co_constraint g_Triv c phi) R) /\
+    (forall G0 D0 p1 p2 R (H : Iso G0 D0 p1 p2 R),
           forall G D A1 A2 T R' F c,
             G0 = (F ++ (c ~ Co (Eq A1 A2 T R') ) ++ G)
             -> DefEq G D A1 A2 T R'
             -> Iso (map (co_subst_co_sort g_Triv c) F ++ G) (union D (remove c D0))
                     (co_subst_co_constraint g_Triv c p1)
-                    (co_subst_co_constraint g_Triv c p2)) /\
+                    (co_subst_co_constraint g_Triv c p2) R) /\
     (forall G0 D0 A B T R'' (H : DefEq G0 D0 A B T R''),
         forall G D F c A1 A2 T1 R',
           G0 = (F ++ (c ~ Co (Eq A1 A2 T1 R') ) ++ G)
@@ -426,7 +426,8 @@ Proof.
   - eapply E_Conv; eauto 3.
   -  have h0: Typing nil a A R by eapply toplevel_closed; eauto.
     erewrite (tm_subst_co_fresh_1 _ h0); eauto.
-  - eapply E_TyCast; try eapply DefEq_weaken_available; eauto.
+(*   - eapply E_TyCast; try eapply DefEq_weaken_available; eauto. *)
+  - eauto.
   - apply (E_Wff _ _ _  (co_subst_co_tm g_Triv c A)); eauto 3.
   - apply E_PropCong; eauto 3.
   - eapply E_CPiFst; eauto 3.
@@ -447,13 +448,13 @@ Proof.
          pose K := DefEq_weakening.
          apply (K _ _ _ _ _ _ H1); eauto 2.
          eapply H; eauto 2. auto.
-      ++ move : (Typing_context_fv H8) => ?. split_hyp. auto.
-      ++ move : (Typing_context_fv H10) => ?. split_hyp. auto.
-      ++ move: (Typing_context_fv H8) => ?. split_hyp. auto.
+      ++ move : (Typing_context_fv H12) => ?. split_hyp. auto.
+      ++ move : (Typing_context_fv H11) => ?. split_hyp. auto.
+      ++ move: (Typing_context_fv H10) => ?. split_hyp. auto.
     + have: Ctx ([(c1, Co (Eq A1 A2 T1 R'))] ++ G0). by apply (Ctx_strengthen _ F); auto.
       move => h2.
       have: Ctx G0 by eapply Ctx_strengthen; eauto. move => h3.
-      have: PropWff G0 (Eq a b A R). eapply binds_to_PropWff; eauto 1. move => h4.
+      have: PropWff G0 (Eq a b A R) Phm . eapply binds_to_PropWff; eauto 1. move => h4.
       inversion h4. subst. clear h4.
       have: c1 `notin` dom G0. inversion h2; auto.
       move => Fr1.
@@ -463,8 +464,8 @@ Proof.
       eapply binds_app_3; eauto 1.
       eauto.
       all:
-        move: (Typing_context_fv H5) => ?;
         move: (Typing_context_fv H7) => ?;
+        move: (Typing_context_fv H8) => ?;
         split_hyp;
         unfold "[<=]" in *; eauto.
   - eauto.
@@ -482,7 +483,7 @@ Proof.
     eauto 2.
   - eapply E_IsoSnd; eauto 1.
     eapply H; eauto.
-  - eapply E_CastCong; eauto.
+(*   - eapply E_CastCong; eauto. *)
   - induction F; done.
   - induction F; try done.
     destruct a.
@@ -507,6 +508,7 @@ Proof.
       * apply (H _ D _ _ A1 A2 T R'); auto.
       * inversion H4; subst; clear H4.
          apply (H0 G0 D A1 A2 T R' F c1); auto.
+         Unshelve. all: auto.
 Qed.
 
 Lemma Typing_co_subst:
@@ -586,9 +588,8 @@ Qed.
 
 Lemma E_Pi_exists : forall x (G : context) (rho : relflag) (A B : tm) R R',
       x `notin` dom G \u fv_tm_tm_tm B
-      -> Typing ([(x, Tm A R)] ++ G) (open_tm_wrt_tm B (a_Var_f x)) a_Star R
-      -> Typing G A a_Star R
-      -> SubRole R R'
+      -> Typing ([(x, Tm A R)] ++ G) (open_tm_wrt_tm B (a_Var_f x)) a_Star R'
+      -> Typing G A a_Star R'
       -> Typing G (a_Pi rho A R B) a_Star R'.
 Proof.
   intros.
@@ -602,9 +603,8 @@ Qed.
 Lemma E_Abs_exists :  forall x (G : context) (rho : relflag) (a A B : tm) R R',
     x `notin` fv_tm_tm_tm a \u fv_tm_tm_tm B
     -> Typing ([(x, Tm A R)] ++ G) (open_tm_wrt_tm a (a_Var_f x)) (open_tm_wrt_tm B (a_Var_f x)) R'
-    -> Typing G A a_Star R
+    -> Typing G A a_Star Phm
     -> RhoCheck rho x (open_tm_wrt_tm a (a_Var_f x))
-    -> SubRole R R'
     -> Typing G (a_UAbs rho R a) (a_Pi rho A R B) R'.
 Proof.
   intros.
