src/FcEtt/ext_weak.v
@@ -55,8 +55,8 @@ Ltac E_pick_fresh x :=
 (* Can replace set with an equivalent *)
 Lemma respects_atoms_eq_mutual :
   (forall G a A R,     Typing  G a A R       -> True) /\
-  (forall G phi,     PropWff G phi       -> True) /\
-  (forall G D p1 p2, Iso G D p1 p2 -> forall D', D [=] D' -> Iso G D' p1 p2) /\
+  (forall G phi R,     PropWff G phi R      -> True) /\
+  (forall G D p1 p2 R , Iso G D p1 p2 R -> forall D', D [=] D' -> Iso G D' p1 p2 R) /\
   (forall G D A B T R,   DefEq G D A B T R -> forall D', D [=] D' -> DefEq G D' A B T R) /\
   (forall G,           Ctx G           -> True).
 Proof.
@@ -107,9 +107,9 @@ Ltac binds_cons :=
 
 Lemma strengthen_available_noncovar:
   (forall G1  a A R,    Typing G1 a A R -> True) /\
-  (forall G1  phi,    PropWff G1 phi -> True) /\
-  (forall G1 D p1 p2, Iso G1 D p1 p2 -> forall x, not (exists phi, binds x (Co phi) G1) ->
-                 Iso G1 (remove x D) p1 p2) /\
+  (forall G1  phi R,    PropWff G1 phi R -> True) /\
+  (forall G1 D p1 p2 R, Iso G1 D p1 p2 R -> forall x, not (exists phi, binds x (Co phi) G1) ->
+                 Iso G1 (remove x D) p1 p2 R) /\
   (forall G1 D A B A1 R, DefEq G1 D A B A1 R ->  forall x, not (exists phi, binds x (Co phi) G1) ->
                  DefEq G1 (remove x D) A B A1 R) /\
   (forall G1 ,        Ctx G1 -> True).
@@ -138,14 +138,15 @@ Proof.
   assert (Tm A' R' = Co phi). eapply binds_unique; eauto.
   by eauto using DefEq_Ctx, Ctx_uniq. symmetry.
   auto.
+  Unshelve. exact Nom.
 Qed.
 
 (* ----- *)
 
 Lemma weaken_available_mutual:
   (forall G1  a A R,   Typing G1 a A R -> True) /\
-  (forall G1  phi,   PropWff G1 phi -> True) /\
-  (forall G1 D p1 p2, Iso G1 D p1 p2 -> forall D', D [<=] D' -> Iso G1 D' p1 p2) /\
+  (forall G1  phi R,   PropWff G1 phi R -> True) /\
+  (forall G1 D p1 p2 R, Iso G1 D p1 p2 R -> forall D', D [<=] D' -> Iso G1 D' p1 p2 R) /\
   (forall G1 D A B T R,   DefEq G1 D A B T R -> forall D', D [<=] D' -> DefEq G1 D' A B T R) /\
   (forall G1 ,       Ctx G1 -> True).
 Proof.
@@ -161,9 +162,9 @@ Qed.
 
 Lemma remove_available_mutual:
   (forall G1  a A R,   Typing G1 a A R -> True) /\
-  (forall G1  phi,   PropWff G1 phi -> True) /\
-  (forall G1 D p1 p2, Iso G1 D p1 p2 ->
-                   Iso G1 (AtomSetImpl.inter D (dom G1)) p1 p2) /\
+  (forall G1  phi R,   PropWff G1 phi R -> True) /\
+  (forall G1 D p1 p2 R, Iso G1 D p1 p2 R ->
+                   Iso G1 (AtomSetImpl.inter D (dom G1)) p1 p2 R) /\
   (forall G1 D A B T R,   DefEq G1 D A B T R ->
                    DefEq G1 (AtomSetImpl.inter D (dom G1)) A B T R) /\
   (forall G1 ,       Ctx G1 -> True).
@@ -207,7 +208,7 @@ Proof.
 Qed.
 
 Lemma Iso_weaken_available :
-  forall G D A B, Iso G D A B -> Iso G (dom G) A B.
+  forall G D A B R, Iso G D A B R -> Iso G (dom G) A B R.
 Proof.
   intros G D. intros.
   remember (AtomSetImpl.inter D (dom G)) as D'.
@@ -222,10 +223,10 @@ Hint Resolve DefEq_weaken_available Iso_weaken_available.
 Lemma typing_weakening_mutual:
   (forall G0 a A R,   Typing G0 a A R ->
      forall E F G, (G0 = F ++ G) -> Ctx (F ++ E ++ G) -> Typing (F ++ E ++ G) a A R) /\
-  (forall G0 phi,   PropWff G0 phi ->
-     forall E F G, (G0 = F ++ G) -> Ctx (F ++ E ++ G) -> PropWff (F ++ E ++ G) phi) /\
-  (forall G0 D p1 p2, Iso G0 D p1 p2 ->
-     forall E F G, (G0 = F ++ G) -> Ctx (F ++ E ++ G) -> Iso (F ++ E ++ G) D p1 p2) /\
+  (forall G0 phi R,   PropWff G0 phi R ->
+     forall E F G, (G0 = F ++ G) -> Ctx (F ++ E ++ G) -> PropWff (F ++ E ++ G) phi R ) /\
+  (forall G0 D p1 p2 R, Iso G0 D p1 p2 R ->
+     forall E F G, (G0 = F ++ G) -> Ctx (F ++ E ++ G) -> Iso (F ++ E ++ G) D p1 p2 R) /\
   (forall G0 D A B T R,   DefEq G0 D A B T R ->
      forall E F G, (G0 = F ++ G) -> Ctx (F ++ E ++ G) -> DefEq (F ++ E ++ G) D A B T R) /\
   (forall G0,       Ctx G0 ->
@@ -238,8 +239,21 @@ Proof.
 
   all: try solve [eapply CON; eauto 2].
   all: try solve [eapply CON; eauto 2; eapply DefEq_weaken_available; eauto 2].
-  all: try solve [E_pick_fresh y; try auto_rew_env; apply_first_hyp; try simpl_env; eauto 3].
-
+  all: try solve [E_pick_fresh y; try auto_rew_env; apply_first_hyp; try simpl_env; eauto 4].
+  idtac.
+  E_pick_fresh y; try auto_rew_env; apply_first_hyp; try simpl_env; eauto 4.
+  econstructor; eauto.
+  move: (H0 _ _ _ eq_refl H2) => p1.
+  inversion p1.
+  eapply E_Wff; eapply E_SubRole; eauto.
+  eapply CON; eauto 2.
+  instantiate (1:= L \u dom (F ++ E ++ G0)) => c h0.
+  eapply (H0 c ltac:(auto) E (c ~ Co (Eq a1 b1 A1 R) ++ F) _ eq_refl); eauto 2.
+  simpl_env.
+  econstructor; eauto 2.
+  move: (H1 _ _ _ eq_refl H5) => p2.
+  inversion p2.
+  eapply E_Wff; eapply E_SubRole; eauto.
   (*
   eapply E_LeftRel with (b:=b)(b':=b'); eauto 2;
     try eapply DefEq_weaken_available; eauto 2.
